examples/TTS_ex.v
@@ -1,0 +1,205 @@
+Require Import TTS.
+Require Import ltacs.
+Require Import String.
+Require Import Coq.Lists.List.
+Import Coq.Lists.List.ListNotations.
+Require Import LTS.
+Require Import IOTS.
+Require Import list_helper.
+Require Import LTS_functions.
+Require Import IOTS.
+Require Import IOTS_ex.
+
+Local Open Scope string.
+
+Definition fig7_t1_LTS : LTS.
+Proof.
+   solve_LTS_rules
+          [0;1;2;3;4]
+          ["but"; "liq";"choc";"theta"]
+          [(1, event "but", 2); (1, event "liq", 0); (1, event "choc", 0);
+           (2, event "liq", 3); (2, event "theta", 0); (2, event "choc", 0);
+           (3, event "theta", 4); (3, event "liq", 0); (3, event "choc", 0);
+           (0, event "liq", 0); (0, event "choc", 0); (0, event "theta", 0);
+           (4, event "liq", 4); (4, event "choc", 4); (4, event "theta", 4)]
+          1.
+Defined.
+
+Definition fig7_t1_SC_LTS : SC_LTS.
+Proof.
+  apply (mkSC_LTS fig7_t1_LTS).
+  unfold strongly_converging. intros s t H. destruct t.
+  - destruct H. unfold not in H. exfalso. apply H. reflexivity.
+  - unfold all_labels_tau in H. destruct H as [_ [H _]].
+    unfold not. intros H'. inversion H'.
+    + subst. proof_absurd_transition H5.
+    + subst. expand_transition H3.
+Defined.
+
+Definition fig7_t1_IOLTS : IOLTS.
+Proof.
+  solve_IOLTS_rules
+    fig7_t1_SC_LTS
+    ["liq";"choc"]
+    ["but"; "theta"].
+Defined.
+
+Definition fig7_t1_IOTS : IOTS.
+Proof.
+  apply (mkIOTS fig7_t1_IOLTS).
+  unfold valid_iots. exists [0;1;2;3;4]. split.
+  - apply der_LTS_r1. apply der_r1. intros s'. simpl q0. split.
+    + intros H. destruct H as [ll H].
+      repeat (
+        induction ll; expand_seq_reachability H; try elem_in_list; auto; clear IHll).
+    + intros H. expand_In H.
+      * exists ["liq"]. proof_seq_reachability [(@nil nat, 0)] (@nil nat).
+      * exists [ ]. proof_seq_reachability (@nil nat) (@nil nat).
+      * exists ["but"]. proof_seq_reachability [(@nil nat, 2)] (@nil nat).
+      * exists ["but"; "liq"].
+        proof_seq_reachability [(@nil nat, 2); (@nil nat, 3)] (@nil nat).
+      * exists ["but"; "liq"; "theta"].
+        proof_seq_reachability [(@nil nat, 2); (@nil nat, 3); (@nil nat, 4)] (@nil nat).
+  - simpl. repeat split; eapply has_reachability_to_some_other_r1;
+    try (proof_seq_reachability [(@nil nat, 0)] (@nil nat)).
+   + proof_seq_reachability [(@nil nat, 3)] (@nil nat).
+   + proof_seq_reachability [(@nil nat, 4)] (@nil nat).
+   + proof_seq_reachability [(@nil nat, 4)] (@nil nat).
+Defined.
+
+
+Ltac try_all list f :=
+  lazymatch list with
+  | [ ] => idtac
+  | ?h :: ?t => f h + try_all t f
+  end.
+
+Ltac create_TTS iots pass_state fail_state theta imp_Li :=
+  apply (mkTTS iots pass_state fail_state theta); try elem_in_list; auto;
+  try (intros l s H; expand_transition H; subst; simpl; split; auto);
+  [
+    unfold ind_deterministic; intros t ls H; inversion H as [? ? H_aux]; subst;
+    clear H; rename H_aux into H;
+    inversion H as [? ? ? H_aux]; subst; clear H; rename H_aux into H;
+    simpl in H; inversion H as [? ? ? ? H_aux]; subst; clear H; rename H_aux into H;
+    intros H' H''; inversion H' as [? ? ? H_aux]; subst; simpl in H_aux;
+    clear H'; rename H_aux into H';
+    apply ind_after_reflect in H';  unfold f_after in H';
+    symmetry_eqv in H';
+    repeat (induction t as [| ? t IHt]; expand_seq_reachability H; auto;
+      simpl f_after' in H';
+      try (apply Equiv_eqLength in H'; auto; apply NoDup_cons; auto;
+           apply NoDup_nil); clear IHt)
+  |
+    intros t; destruct t; intros s H H'; [destruct H; reflexivity |];
+    simpl in H';
+      assert (H_fail:
+        forall s t,
+          ind_seq_reachability fail_state t s iots.(embedded_iolts).(sc_lts).(lts) ->
+          s = fail_state);
+      [ intros s' t' H''; induction t'; expand_seq_reachability H''; auto |];
+      assert (H_pass:
+        forall s t,
+          ind_seq_reachability pass_state t s iots.(embedded_iolts).(sc_lts).(lts) ->
+          s = pass_state);
+      [ intros s' t' H''; induction t'; expand_seq_reachability H''; auto |];
+      expand_seq_reachability H'; auto;
+      repeat (destruct t as [| ? t];
+        try (
+         inversion H' as [ ? ? ? H_empty |];
+         inversion H_empty as [ | ? ? ? ? H_trans ?];
+         subst; expand_transition H_trans; fail);
+        expand_seq_reachability H';
+        try (apply H_pass in H'; inversion H');
+        try (apply H_fail in H'; inversion H'))
+  |
+    intros q H; simpl; expand_In H; vm_compute f_init;
+    try (left; proof_Equiv); right;
+    try_all (imp_Li) ltac:(fun x => (exists x; split; auto; proof_Equiv)) ].
+
+
+Definition fig7_t1_TTS : TTS.
+Proof.
+  create_TTS fig7_t1_IOTS 0 4 "theta" ["but"].
+Defined.
+
+Ltac expand_test_execution_transition H :=
+  let H_trans := fresh "H_trans" in
+  let H_trans' := fresh "H_trans'" in
+  let H_In := fresh "H_In" in
+  let H_eq := fresh "H_eq" in
+    lazymatch type of H with
+    | ind_test_execution_transition _ _ tau _ _ _ _ =>
+        inversion H as [? ? ? ? ? H_trans | |]; subst; expand_transition H_trans
+    | ind_test_execution_transition _ _ (event _) _ _ _ _ =>
+        inversion H as [|
+          ? ? ? ? ? ? ? H_In H_trans H_trans' |
+          ? ? ? ? ? ? H_eq H_trans H_In];
+        subst; try (inversion H_eq); subst; expand_In H_In; subst;
+        expand_transition H_trans; try (expand_transition H_trans')
+    end.
+
+Ltac expand_test_execution_empty_reachability H :=
+  let H_tau := fresh "H_tau" in
+  let H_empty := fresh "H_empty" in
+    inversion H as [ | ? ? ? ? ? ? ? ? H_tau H_empty]; subst;
+    try (expand_test_execution_transition H_tau; subst;
+         expand_test_execution_empty_reachability H_empty; subst).
+
+Ltac expand_test_execution_one_step_reachability H :=
+  let H_empty := fresh "H_empty" in
+  let H_trans := fresh "H_trans" in
+    inversion H as [? ? ? ? ? ? ? ? ? H_empty H_trans]; subst;
+    expand_test_execution_empty_reachability H_empty;
+    expand_test_execution_transition H_trans;
+    clear H_empty H_trans.
+ 
+Ltac expand_test_execution_seq_reachability H :=
+  let H_empty := fresh "H_empty" in
+  let H_one_step := fresh "H_one_step" in
+  let H_seq := fresh "H_seq" in
+    lazymatch type of H with
+    | ind_test_execution_seq_reachability _ _ [ ] _ _ _ _ =>
+        inversion H as [ ? ? ? ? ? ? H_empty |]; subst;
+        expand_test_execution_empty_reachability H_empty; subst; clear H_empty
+    | ind_test_execution_seq_reachability _ _ (_ :: _) _ _ _ _ =>
+        inversion H as [| ? ? ? ? ? ? ? ? ? ? H_one_step H_seq]; subst;
+        expand_test_execution_one_step_reachability H_one_step; subst;
+        expand_test_execution_seq_reachability H_seq; subst; clear H H_one_step;
+        rename H_seq into H
+    | ind_test_execution_seq_reachability _ _ _ _ _ _ _ => idtac
+    | _ => fail "Invalid Hypothesis format"
+    end.
+
+Example k1_passes_t1 : ind_passes fig4_k1_IOTS fig7_t1_TTS.
+Proof.
+  unfold ind_passes. intros sigma i' _ H.
+  unfold ind_test_execution_trace in H. simpl in H.
+  destruct sigma; expand_test_execution_seq_reachability H.
+  destruct sigma; expand_test_execution_seq_reachability H.
+  destruct sigma; expand_test_execution_seq_reachability H.
+  induction sigma; expand_test_execution_seq_reachability H; auto.
+Qed.
+
+Example k3_fails_t1 : ~ ind_passes fig4_k3_IOTS fig7_t1_TTS.
+Proof.
+  unfold ind_passes. unfold ind_test_execution_trace. simpl. intros H.
+  specialize (H ["but"; fig7_t1_TTS.(theta)] 2).
+  apply H;
+  [ unfold ind_test_run; exists 2; right; simpl fail_state;
+    unfold ind_test_execution_trace; simpl q0 |];
+  eapply test_execution_seq_reachability_r2 with (i2 := 2);
+   try (eapply test_execution_one_step_reachability_r1;
+    try (apply test_execution_empty_reachability_r1);
+    apply test_execution_transition_r2; try elem_in_list; apply transition_r1;
+    elem_in_list);
+    apply test_execution_seq_reachability_r2 with (t2 := 0) (i2 := 2);
+    try (apply test_execution_seq_reachability_r1;
+      apply test_execution_empty_reachability_r1);
+    eapply test_execution_one_step_reachability_r1;
+      try (apply test_execution_empty_reachability_r1);
+      apply test_execution_transition_r3; try elem_in_list; auto;
+      apply transition_r1; simpl; elem_in_list.
+Qed.
+
+Local Close Scope string.
